ACTL.v
@@ -1,0 +1,374 @@
+
+Require Export Classical.
+Require Import Coq.Setoids.Setoid.
+
+Section Def.
+
+
+Context {state action : Set} {trans : state -> action -> state -> Prop}
+        {tau : action} {tau_eq : forall  s s', trans s tau s' <->  s = s'}.
+
+     
+
+(******************** path ********************)
+
+CoInductive path : state -> Set :=
+    | nilp s a s' : trans s a s' -> path s
+    | consp s a s' : trans s a s' -> path s' -> path s.
+
+
+
+Inductive run := Run s : path s -> run.
+
+Definition headState (r : run) : state :=
+    match r with Run s _ => s end.
+
+Definition nextState (r : run) : state :=
+    match r with 
+    | Run s p => match p with 
+        | nilp _ _ s' _ => s' 
+        | consp _ _ s' _ _ => s' 
+        end 
+    end.
+
+
+
+
+
+Definition pathOf (r : run) : match r with Run s _ => path s end :=
+    match r with 
+    | Run s p => p
+    end.
+
+Definition headAction (r : run) : action :=
+    match r with 
+    | Run _ p => match p with
+        | nilp _ a _ _ => a
+        | consp _ a _ _ _ => a 
+        end 
+    end.
+ 
+
+(******************** action_formula ********************)
+
+
+
+Inductive action_form :=
+    | any : action_form 
+    | action_ : action -> action_form
+    | not_ : action_form -> action_form
+    | and_ : action_form -> action_form -> action_form.
+
+Definition non := not_ any .  
+
+Fixpoint sata  (a : action) (chi : action_form) : Prop :=
+    match chi with 
+    | any => True 
+    | action_ a' => a = a' 
+    | not_ chi' => ~ sata a chi' 
+    | and_ chi1 chi2 => sata a chi1 /\ sata a chi2
+    end. 
+
+
+
+
+
+
+
+
+
+
+(******************** ACTL ********************)
+
+Inductive Until (f f' : state -> Prop) (chi chi' : action_form) : run -> Prop :=
+    | until_here r : 
+        sata (headAction r) chi' -> f' (nextState r) -> Until f f' chi chi' r
+    | until_there s a s' H p: 
+        sata a chi -> f s' -> Until f f' chi chi' (Run s' p) -> 
+        Until f f' chi chi' (Run s (consp s a s' H p)).
+
+Inductive form :=
+    | top : form 
+    | bot : form 
+    | not : form -> form
+    | and : form -> form -> form 
+    | or : form -> form -> form 
+    | imp : form -> form -> form
+    | exist : formr -> form 
+    | all : formr -> form
+
+with formr :=
+    | until : form -> form -> action_form -> action_form -> formr.
+
+
+
+
+Scheme form_mut := Induction for form Sort Prop 
+with formr_mut := Induction for formr Sort Prop.
+
+
+
+Fixpoint sat (f : form) (s : state)  : Prop :=
+    match f with 
+    | top => True
+    | bot => False
+    | not f => ~ (sat f) s
+    | and f1 f2 => sat f1 s /\ sat f2 s 
+    | or f1 f2 => sat f1 s \/ sat f2 s
+    | imp f1 f2 => sat f1 s -> sat f2 s 
+    | exist f => exists r' , headState r' = s /\ satr f r'
+    | all f => forall r', headState r' = s -> satr f r'
+    end
+
+with satr (f : formr) (r : run) : Prop :=
+    match f with 
+    | until f1 f2 chi chi' =>  sat f1 (headState r)  /\  Until (sat f1) (sat f2) chi chi' r
+    end.
+
+End Def.
+
+(******************** derived operation ********************)
+
+
+Notation "⊤" := top.
+Notation "⊥" := bot.
+Notation "¬ f" := (not f)(at level 10).
+Notation "f ∧ f'" := (and f f')(at level 20).
+Notation "f ∨ f'" := (or f f')(at level 20).
+Notation "f → f'" := (imp f f')(at level 30).
+
+Notation "f [ chi ]  'U'  [ chi' ] f'" := (until f f' chi chi')(at level 50).
+Notation "f 'U' f'" := (f [any] U [any] f')(at level 50).
+Notation "[ chi ]  'U'  [ chi' ] f'" := (⊤ [chi] U [chi'] f')(at level 50).
+
+Notation "'E' p" := (exist p)(at level 50).
+Notation "'A' p" := (all p)(at level 50).
+Notation "'EX' [ chi ] f" := (E (⊤ [non] U [chi] f))(at level 50, chi at level 5).
+Notation "'AX' [ chi ] f" := (A (⊤ [non] U [chi] f))(at level 50, chi at level 5).
+Notation "'EF' [ chi ] f" := (E (⊤ [any] U [chi] f))(at level 50, chi at level 5).
+Notation "'AF' [ chi ] f" := (A (⊤ [any] U [chi] f))(at level 50, chi at level 5).
+
+
+
+
+
+
+
+Section theorems.
+
+Context {state action : Set} {trans : state -> action -> state -> Prop}
+        {tau : action} {tau_eq : forall  s s', trans s tau s' <->  s = s'}.
+
+
+Notation "s |= f" := (@sat state action trans f s)(at level 80).
+Notation "|= f" := (forall s, s |= f)(at level 80).
+Notation τ := (action_ tau).
+Notation "< chi > f" := (E (⊤ [τ] U [chi] f))(at level 50, chi at level 5).
+Notation "[ chi ] f" := (¬ <chi> ¬ f)(at level 50, chi at level 5).
+Notation "'EX' f" := (<any> f)(at level 50).
+Notation "'AX' f" := ([any] f)(at level 50).
+Notation "'EF' f" := (f ∨ EF [any] f)(at level 50).
+Notation "'AF' f" := (f ∨ AF [any] f)(at level 50).
+Notation "'EG' f" := (¬ AF ¬ f)(at level 50).
+Notation "'AG' f" := (¬ EF ¬ f)(at level 50).
+
+Notation "f 'EU' f'" := (f' ∨ (f ∧ (EX (E (f U f')))))(at level 50).
+Notation "f 'AU' f'" := (f' ∨ (f ∧ (AX (A (f U f')))))(at level 50).
+Notation "f 'EW' f'" := (¬ ((¬ f') AU ((¬ f) ∧ (¬ f'))))(at level 50).
+Notation "f 'AW' f'" := (¬ ((¬ f') EU ((¬ f) ∧ (¬ f'))))(at level 50).
+
+
+Theorem tau_refl s :
+    trans s tau s.
+Proof.
+    apply tau_eq; auto.
+Qed.   
+
+
+Theorem dia_spec f s chi:
+    s |= <chi> f <-> 
+    exists a s', sata a chi /\ trans s a s' /\ s' |= f.
+Proof.
+    split.
+    +   destruct f;
+        try (
+            intro H; induction H as [r [Hr [_ HU]]]; subst;
+            induction HU; subst; simpl in *; subst; 
+                try (destruct r, p; simpl in *; exists a, s'; repeat split; auto);
+                assert (s = s') by (apply tau_eq; auto); subst s'; auto
+        ).
+        {
+            intro H; induction H as [r [Hr [_ HU]]]; subst.
+            induction HU; subst; simpl in *; subst. 
+                try (induction H0; destruct r, p; simpl in *; exists a, s'; repeat split; auto).
+                assert (s = s') by (apply tau_eq; auto); subst s'; auto.
+        }               
+    +   intro H; induction H as [a [s' [H_ [Ht Hf]]]].
+        unfold sat; simpl.
+        exists (Run s (nilp s a s' Ht)); repeat split; constructor; auto.
+Qed.  
+
+
+
+
+Theorem box_spec f s chi :  
+    s |= [chi] f <->
+    forall r : run (trans := trans),
+        headState r = s ->
+        sata (headAction r) chi -> 
+        trans (headState r) (headAction r) (nextState r) -> 
+        (nextState r) |= f.
+Proof.
+    split.
+    +   destruct f;
+            unfold sat; intros H r Hr Ha Ht;
+            apply not_ex_all_not with (n := r) in H;
+            apply not_and_or in H;
+            induction H; try (case (H Hr)); subst;
+            apply not_and_or in H;
+            induction H; apply NNPP; intro F; apply H; auto; clear H;
+            destruct r, p; simpl in *; constructor; simpl; auto.
+    +   destruct f; auto;
+            unfold sat; intros H F;
+            induction F as [r [Hr [_ HU]]];
+            induction HU; auto; simpl in *; subst;
+                try (apply H1; clear H1; apply H; auto; destruct r, p; auto);
+                try (assert (s = s') by (apply tau_eq; auto); subst s'; auto).
+            apply (H r ); auto; destruct r, p; auto.
+Qed.   
+
+Inductive belong : run (trans := trans) -> state -> Prop :=
+    | belong_here r s : headState r = s -> belong r s 
+    | belong_next r s : nextState r = s -> belong r s 
+    | belong_there s a s' H p s'': 
+        belong (Run s' p) s'' -> belong (Run s (consp s a s' H p)) s''.
+
+Theorem EF_spec f s :
+    s |= EF f <-> 
+        exists (r : run (trans := trans)) s', 
+            headState r = s /\ belong r s' /\ s' |= f.
+Proof.
+    split; unfold sat; intro; fold (sat (trans := trans)) in *.
+    +   induction H; auto.
+        *   exists (Run s  (nilp s tau s (tau_refl s))), s; 
+            repeat split; try constructor; auto.
+        *   induction H as [r [Hr [_ HU]]]; subst.
+            induction HU.
+            -   exists r, (nextState r); repeat split; auto.
+                destruct r, p; constructor 2; auto.
+            -   simpl.
+                induction IHHU as [r [s'' [Hr [Hs'' Hf]]]] .
+                destruct r; simpl in *; subst s0.                
+                exists (Run s (consp s a s' H p0)), s''; repeat split; auto.
+                constructor 3; auto.
+    +   induction H as [r [s' [Hr [Hs Hf]]]]; subst.
+        induction Hs; subst; auto; right; simpl in *.
+        -   exists r; repeat split.
+            constructor; unfold sata; auto.
+        -   apply IHHs in Hf.
+            induction Hf; auto.
+            *   exists (Run s (nilp s a s' H)); repeat split.
+                constructor; try unfold sata; auto.
+            *   induction H0 as [r [Hr [_ HU]]].
+                destruct r; simpl in Hr; subst s0.
+                exists (Run s (consp s a s' H p0)); repeat split.
+                constructor 2; try unfold sata; auto.
+Qed. 
+
+
+Theorem AF_spec f s :
+    s |= AF f <->
+        (forall r, headState r = s ->
+        (exists s', belong r s' /\ s' |= f)).
+Proof.
+    split; unfold sat; intro; fold (sat (trans := trans)) in *.
+    +   intros r Hr.
+        induction H.
+        -   exists s; split; auto; constructor; auto.
+        -   apply H in Hr; clear H.
+            induction Hr as [_].
+            induction H.
+            *   exists (nextState r); split; auto.
+                constructor 2; auto.
+            *   induction IHUntil as [s'' [Hs'' Hf]].
+                exists s''; split; auto.
+                constructor 3; auto.
+    +   specialize (H (Run s (nilp s tau s (tau_refl s))) (eq_refl s)).
+        induction H as [s' [Hs Hf]].
+        inversion Hs; subst; auto.
+Qed.    
+
+Theorem axiomK f f' :
+    |= (AX (f → f')) → ((AX f) → (AX f')).
+Proof.
+    unfold sat; intros; fold (sat (trans := trans)) in *.
+    intro F; induction F as [r [Hr [_ HU]]].
+    induction HU.
+    +   apply H0; exists r; repeat split; auto.
+        constructor; try unfold sata; auto; intro F.
+        apply H; exists r; repeat split; auto.
+        constructor; try unfold sata; auto.
+    +   simpl in *; subst s0 a.
+        apply IHHU; symmetry; apply tau_eq; auto.
+Qed.  
+
+Theorem axiomAXEX f :
+    |= (AX f) → (EX f).
+Proof.
+    unfold sat; intros s H; fold (sat (trans := trans)) in *.
+    remember (Run s (nilp s tau s (tau_refl s))).
+    apply not_ex_all_not with (n := r) in H.
+    apply not_and_or in H.
+    induction H; simpl in *.
+    +   contradiction H; subst; auto.
+    +   apply not_and_or in H; induction H; [apply NNPP; intro F; apply H; auto|].
+        apply NNPP; intro F; apply H; constructor; unfold sata; auto; simpl.
+        intro F_; apply F.
+        exists r; subst; repeat split; constructor; unfold sata; auto.
+Qed.        
+
+Ltac  satisfy := unfold sat; fold (sat (trans := trans)).
+
+Theorem axiomAX f :
+    |= f -> |= AX f.
+Proof.
+    satisfy; intros H s F.
+    induction F as [r [Hr [_ HU]]].
+    induction HU; eauto; simpl in *; subst.
+    apply IHHU; symmetry; apply tau_eq; auto.
+Qed.
+
+
+
+Theorem AU_ind f g h :
+    |= g → h -> (|= f → ((AX h) → h)) -> |= (f AU g) → h.
+Proof.
+    satisfy; intros IH IH' s H.
+    induction H; eauto.
+    induction H.
+    apply (IH' s H); clear IH'.
+    intro F; apply H0; clear H0.
+    induction F as [r [Hr [_ HU]]].    
+    induction HU; simpl in *; subst.
+    -   exists r; repeat split; auto.
+        constructor; auto; intro F.
+        specialize (F 
+            (Run (nextState r) (nilp (nextState r) tau (nextState r) (tau_refl (nextState r))))
+            (eq_refl (nextState r))
+        ); simpl in F; induction F.
+        inversion H3; simpl in *; auto.
+    -   rewrite tau_eq in H0; symmetry in H0; auto.
+Qed.  
+
+Theorem EU_ind f g h :
+    |= g → h -> (|= f → ((EX h) → h)) -> |= (f EU g) → h.
+Proof.
+Abort.
+            
+Theorem AU_intro f g :
+    |= g →  (f AU g).
+Proof.
+    satisfy; intros s H; left; auto.
+Qed.
+
+End theorems.
